rustfrontend/BorrowCheckSound.v
@@ -9,8 +9,8 @@ Require Import Globalenvs.
 Require Import Smallstep SmallstepLinking SmallstepLinkingSafe.
 Require Import LanguageInterface CKLR Invariant.
 Require Import Rusttypes Rustlight Rustlightown.
-Require Import RustIRspec.
 Require Import RustOp RustIR RustIRcfg Rusttyping.
+Require Import RustIRspec.
 Require Import Errors.
 Require Import Listmisc.
 (* move checking *)
@@ -20,11 +20,9 @@ Require Import MoveChecking.
 Require Import RegionLiveness BorrowCheckDomain.
 Require Import BorrowCheckPolonius BorrowCheck BorrowCheckInv.
 
-
 Import ListNotations.
 
 Local Open Scope error_monad_scope.
-
 
 
 Section ADT_ENV.
@@ -35,6 +33,8 @@ Notation footprint := (@footprint ame).
 Notation fp_map := (@fp_map ame).
 Notation fp_graph := (@fp_graph ame).
 Notation get_owner_path_map := (@get_owner_path_map ame).
+Notation cont := (@cont ame).
+Notation state := (@state ame).
 
 Section BORROW_CHECK.
 
@@ -68,14 +68,14 @@ Hypothesis COMP_NOREP: forall id co, ce ! id = Some co -> list_norepet (name_mem
 
 Let INIT_AN : Type := (PMap.t IM.t * PMap.t IM.t * PathsMap.t).
 
-Let move_check_stmt (ae: INIT_AN) body cfg s ts := match_stmt get_init_info ae (move_check_stmt ce) (check_cond_expr ce) body cfg s ts.
+Let move_check_stmt_spec (ae: INIT_AN) body cfg s ts := match_stmt get_init_info ae (move_check_stmt ce) (check_cond_expr ce) body cfg s ts.
 
 (* Result of the loans-flow analysis and the result of the borrow
 checking *)
 
 Let LOANS_AN : Type := (PMap.t RegionSet.t * PMap.t LoansEnv.t).
 
-Let borrow_check_stmt (ae: LOANS_AN) regs f cfg s ts := match_stmt (get_borck_result regs f cfg) ae (borrow_check_stmt f) borrow_check_cond_expr f.(fn_body) cfg s ts.
+Let borrow_check_stmt_spec (ae: LOANS_AN) regs f cfg s ts := match_stmt (get_borck_result regs f cfg) ae (borrow_check_stmt f) borrow_check_cond_expr f.(fn_body) cfg s ts.
 
 (** Over-approximation of the borrow analysis. Note that this
 definition is not specific to which borrow checking algorithms you
@@ -85,46 +85,79 @@ of the program. *)
 
 (* We also need to know that generic region this path locates
 at....  *)
-Definition extern_loc_region (fpm: fp_map) (ph: path) : option origin :=
+Definition extern_loc_region (orgm: PTree.t (option origin)) (ph: path) : option origin :=
   let (id, pj) := ph in
-  match fpm ! id with
-  | Some (_, _, r, _, _) =>
+  match orgm ! id with
+  | Some r =>
       r
   | _ => None
   end.
 
-Definition loan_approx (fpm: fp_map) (ln: loan) (ph: path) : Prop :=
-  match ln, extern_loc_region fpm ph with
-  | Lintern _ p, None =>
+Definition mutability_match (ref_mut loan_mut: mutkind) : Prop :=
+  match ref_mut, loan_mut with
+  | Mutable, Mutable => True
+  (* If this reference is immutable reference, than we do not need to
+  care the how we create this loan *)
+  | Immutable, _ => True
+  | _, _ => False
+  end.
+
+Definition loan_approx (orgm: PTree.t (option origin)) (ln: loan) (ref_mut: mutkind) (ph: path) : Prop :=
+  match ln, extern_loc_region orgm ph with
+  | Lintern loan_mut p, None =>
+      (** Note: mut is the precise mutability of the reference we are focusing. *)
       (* TODO: maybe we should use path uniformly *)
       let (id1, pj1) := path_of_place p in
       let (id2, pj2) := ph in
-      id1 = id2 /\ projections_contain pj1 pj2 = true
+      id1 = id2 /\ projections_contain pj1 pj2 = true /\ mutability_match ref_mut loan_mut
   | Lextern org1, Some org2 =>
       org1 = org2 
   | _, _ => False
   end.
 
-Definition sound_loan_analysis ce (le: LOrgEnv.t) (fpm: fp_map) : Prop :=
-  forall ph owner_ph opt_ph vs1 vs2 mut b ofs r ty ls,
+Definition loans_approx_views (orgm: PTree.t (option origin)) (ls: LoanSet.t) (ref_mut: mutkind) (vs: views) : Prop :=
+  forall vph, In vph vs ->
+         exists ln, LoanSet.In ln ls /\ loan_approx orgm ln ref_mut vph.
+
+Definition fpm_to_orgm (fpm: fp_map) : PTree.t (option origin) :=
+  PTree.map1 (fun '(_,_,r,_,_) => r) fpm.
+
+
+Definition sound_loan_analysis ce (live: RegionSet.t) (le: LOrgEnv.t) (fpm: fp_map) : Prop :=
+  forall ph owner_ph opt_ph vs1 vs2 mut b ofs r ty
     (* If we make these two get_xxx as assumptions, how can we use
     this approximation property to prove progress, i.e., how to prove
     these two assumptions. For example, when we prove the progress in
     eval_pexpr on Eplace, the two get functions can be proved to make
     progress by using induciton, this approximation property and
     property about "all owners pointed by reference is init" *)
-    get_owner_path_map ph fpm = OK (owner_ph, vs1) ->
-    get_owner_footprint_map owner_ph fpm = OK (fp_ref mut b ofs opt_ph vs2) ->
-    wt_path ce (fpm_to_tenv fpm) ph = OK (Treference r mut ty) ->
-    (* We use loans map to tell if r is live or not instead of using
-    the liveness set because we need the loans set of this region *)
-    LOrgEnv.get r le = Live ls ->
+    (GET_PH: get_owner_path_map ph fpm = OK (owner_ph, vs1))
+    (GET_FP: get_owner_footprint_map owner_ph fpm = OK (fp_ref mut b ofs opt_ph vs2))
+    (WTPH: wt_path ce (fpm_to_tenv fpm) ph = OK (Treference r mut ty))
+    (LIVE_REG: RegionSet.In r live),
+    (* live region contains valid loans *)
+    exists ls, LOrgEnv.get r le = Live ls
     (* Safety: this reference is not invalidated *)
-    (exists rph, opt_ph = Some rph)
-    /\ (* Approximation: all (mutable) paths in the vs2 are
-    approximated in the loans map *)
-      (forall vph, In vph vs2 ->
-              exists ln, LoanSet.In ln ls /\ loan_approx fpm ln vph).
+    /\ (exists rph, opt_ph = Some rph)
+    (* Approximation: all (mutable) paths in the vs2 are approximated
+    in the loans map *)
+    /\ loans_approx_views (fpm_to_orgm fpm) ls mut vs2.
+
+(* For temporary values *)
+Definition sound_loan_analysis_footprint ce (le: LOrgEnv.t) (fpm: fp_map) (fp: footprint) (ty: type) : Prop :=
+  forall phl opt_ph vs mut b ofs r ty
+    (GET_FP: get_reachable_footprint fpm phl fp = OK (fp_ref mut b ofs opt_ph vs))
+    (WT_PROJS: wt_projections ce ty phl = OK (Treference r mut ty)),
+    (* live region contains valid loans *)
+    exists ls, LOrgEnv.get r le = Live ls
+    (* Safety: this reference is not invalidated *)
+    /\ (exists rph, opt_ph = Some rph)
+    (* Approximation: all (mutable) paths in the vs are approximated
+    in the loans map *)
+    /\ loans_approx_views (fpm_to_orgm fpm) ls mut vs.
+
+Definition sound_loan_analysis_footprint_list ce (le: LOrgEnv.t) (fpm: fp_map) (fpl: list footprint) (tyl: list type) : Prop :=
+  Forall2 (sound_loan_analysis_footprint ce le fpm) fpl tyl.
 
 
 (** Over-approximation of the init analysis *)
@@ -151,65 +184,331 @@ Definition sound_init_analysis (fpm: fp_map) (init uninit universe: PathsMap.t) 
 
 (** state invariants *)
 
-Inductive sound_state: state -> Prop :=
-| sound_regular_state: forall f cfg entry maybeInit maybeUninit universe s ts pc next cont brk nret k fpm mayinit mayuninit live LoansEnv loans_env ns sup
-    (* The init and loans-flow analysis results *)
+Inductive sound_cont: INIT_AN -> LOANS_AN -> function -> rustcfg -> cont -> cfg_kinfo -> Prop :=
+| sound_Kstop: forall init_an loans_an f cfg nret
+    (RET: cfg ! nret = Some Iend),
+    sound_cont init_an loans_an f cfg Kstop (mk_cfg_kinfo nret None None nret)
+| sound_Kseq: forall init_an loans_an f cfg s k pc next cont brk nret
+    (MCK_STMT: move_check_stmt_spec init_an f.(fn_body) cfg s s (mk_cfg_info pc next cont brk nret))
+    (BORCK_STMT: borrow_check_stmt_spec loans_an (regset_fun f) f cfg s s (mk_cfg_info pc next cont brk nret))
+    (MCONT: sound_cont init_an loans_an f cfg k (mk_cfg_kinfo next cont brk nret)),
+    sound_cont init_an loans_an f cfg (Kseq s k) (mk_cfg_kinfo pc cont brk nret)
+| sound_Kloop: forall init_an loans_an f cfg s k body_start loop_jump_node exit_loop nret contn brk
+    (START: cfg ! loop_jump_node = Some (Inop body_start))
+    (MCK_STMT: move_check_stmt_spec init_an f.(fn_body) cfg s s (mk_cfg_info body_start loop_jump_node (Some loop_jump_node) (Some exit_loop) nret))
+    (BORCK_STMT: borrow_check_stmt_spec loans_an (regset_fun f) f cfg s s (mk_cfg_info body_start loop_jump_node (Some loop_jump_node) (Some exit_loop) nret))
+    (MCONT: sound_cont init_an loans_an f cfg k (mk_cfg_kinfo exit_loop contn brk nret)),
+    sound_cont init_an loans_an f cfg (Kloop s k) (mk_cfg_kinfo loop_jump_node (Some loop_jump_node) (Some exit_loop) nret)
+| sound_Kcall: forall init_an loans_an f1 cfg k nret f2 p fpm ns inout_params
+    (MSTK: sound_stacks (Kcall p f2 inout_params ns fpm k))
+    (RET: cfg ! nret = Some Iend),
+    (* (WFOWN: wf_own_env e ce own), *)
+    sound_cont init_an loans_an f1 cfg (Kcall p f2 inout_params ns fpm k) (mk_cfg_kinfo nret None None nret)
+
+with sound_stacks : cont -> Prop :=
+| sound_stacks_stop:
+    sound_stacks Kstop
+| sound_stacks_call: forall f nret cfg pc contn brk k p maybeInit maybeUninit universe entry mayinit mayuninit live loans_env LoansEnv mayinit0 mayuninit0 inout_params fpm ns
     (INITAN: InitAnalysis.analyze ce f cfg entry = OK (maybeInit, maybeUninit, universe))
     (LOANSAN: loans_flow_analyze ce f cfg entry = OK (live, LoansEnv))
-    (* The result of move checking and borrow checking *)
-    (MCK_STMT: move_check_stmt (maybeInit, maybeUninit, universe) f.(fn_body) cfg s ts (mk_cfg_info pc next cont brk nret))
-    (BORCK_STMT: borrow_check_stmt (live, LoansEnv) (regset_fun f) f cfg s ts (mk_cfg_info pc next cont brk nret))
     (* The init set and loans environment of the current pc *)
     (IM: get_IM_state maybeInit!!pc maybeUninit!!pc (Some (mayinit, mayuninit)))
     (LOANS_ST: LoansEnv!!pc = LoansEnv.State loans_env)
     (* Invariant for continuation *)
-    (* (CONT: sound_cont (maybeInit, maybeUninit, universe) (live, LoansEnv) f cfg k (mk_cfg_kinfo next cont brk nret) bor_stk fpf) *)
-    (*Over-approximation of the move checking. *)
+    (CONT: sound_cont (maybeInit, maybeUninit, universe) (live, LoansEnv) f cfg k (mk_cfg_kinfo pc contn brk nret))
+    (* may(un)init0 are the intermediate state of this function call
+    statement before initializing p *)
+    (MAY_INIT: mayinit = add_place universe p mayinit0)
+    (MAY_UNINIT: mayuninit = remove_place p mayuninit0)
+    (* we need to maintain this invariant for p's evaluation when
+    function return *)
+    (DOM: dominators_must_init mayinit0 mayuninit0 universe p = true)
+    (** Invariant of the move checking. TODO: it is not correct
+    because we may pass some reference passed locations out. Maybe we
+    can label those locations instead of passing them out? *)
+    (INIT_APPRO: sound_init_analysis fpm mayinit0 mayuninit0 universe)
+    (* Invariant of the borrow checking *)
+    (BORROW_APPRO: sound_loan_analysis ce (live!!pc) loans_env fpm),
+    sound_stacks (Kcall p f inout_params ns fpm k).
+
+
+Inductive sound_state: state -> Prop :=
+| sound_regular_state: forall f cfg entry maybeInit maybeUninit universe s pc next cont brk nret k fpm mayinit mayuninit live LoansEnv loans_env ns sup
+    (* The init and loans-flow analysis results *)
+    (INITAN: InitAnalysis.analyze ce f cfg entry = OK (maybeInit, maybeUninit, universe))
+    (LOANSAN: loans_flow_analyze ce f cfg entry = OK (live, LoansEnv))
+    (* The result of move checking and borrow checking *)
+    (MCK_STMT: move_check_stmt_spec (maybeInit, maybeUninit, universe) f.(fn_body) cfg s s (mk_cfg_info pc next cont brk nret))
+    (BORCK_STMT: borrow_check_stmt_spec (live, LoansEnv) (regset_fun f) f cfg s s (mk_cfg_info pc next cont brk nret))
+    (* The init set and loans environment of the current pc *)
+    (IM: get_IM_state maybeInit!!pc maybeUninit!!pc (Some (mayinit, mayuninit)))
+    (LOANS_ST: LoansEnv!!pc = LoansEnv.State loans_env)
+    (* Invariant for continuation *)
+    (CONT: sound_cont (maybeInit, maybeUninit, universe) (live, LoansEnv) f cfg k (mk_cfg_kinfo next cont brk nret))
+    (* Over-approximation of the move checking. *)
     (INIT_APPRO: sound_init_analysis fpm mayinit mayuninit universe)
     (* Over-approximation of the borrow checking *)
-    (BORROR_APPRO: sound_loan_analysis ce loans_env fpm),
-    sound_state (State f s k ns fpm sup).
-
-
-| sound_dropstate: forall id co fp b ofs st m membs k fpf bor_stk MP fpm ph
-    (CO: ce ! id = Some co)
-    (RANGE: Ptrofs.unsigned ofs + co_sizeof co <= Ptrofs.max_unsigned)
-    (* The location of the dropped place *)
-    (GFP: get_owner_loc_footprint_map ph fpm = Some (b, Ptrofs.unsigned ofs, fp))
-    (* drop_member_footprint says that fp matches (co, st, membs) *)
-    (DROPMEMB: drop_member_footprint id co fp st membs)
-    (CONT: sound_drop_cont k bor_stk (fpf_func fpm fpf))
-    (** We cannot remove the element from fpl because it would make the
-    location (b, ofs) not freeable anymore! *)
-    (* fpl1 is the locations that have been dropped *)
-    (COHERENT: coherent_fpf ce (fpf_func fpm fpf) MP)
-    (MPRED: m |= MP),
-    (* (ACC: rsw_acc w (rsw sg flat_fp m Hm)) *)
-    sound_state (Dropstate id (Vptr b ofs) st membs k bor_stk m)
-| sound_callstate: forall vf fd orgs org_rels tyargs tyres cconv m fpl args fpf k bor_stk VMP MP
-    (FUNC: Genv.find_funct ge vf = Some fd)
+    (BORROW_APPRO: sound_loan_analysis ce (live!!pc) loans_env fpm),
+    sound_state (State f s k ns fpm sup)
+| sound_callstate: forall fun_id fd orgs org_rels tyargs tyres cconv args k inout_fpm sup
+    (FINDF: ge.(genv_defmap) ! fun_id = Some (Gfun fd))
     (FUNTY: type_of_fundef fd = Tfunction orgs org_rels tyargs tyres cconv)
     (* arguments are semantics well typed *)
-    (WTVAL_LIST: sem_wt_val_list ce fpl args VMP)
+    (* (WTVAL_LIST: sem_wt_val_list ce fpl args VMP) *)
     (* Used in assign_loc_sound in function entry proof *)
-    (ANORM: val_casted_list args tyargs)
-    (WTFP: list_forall2 (wt_footprint ce) (type_list_of_typelist tyargs) fpl)
-    (COHERENT: coherent_fpf ce fpf MP)
-    (MPRED: m |= VMP ** MP)
-    (STK: sound_stacks k bor_stk fpf),
+    (* (WTFP: list_forall2 (wt_footprint ce) (type_list_of_typelist tyargs) fpl) *)
+    (STK: sound_stacks k),
     (** TODO: borrow check invariant is missing at function call *)
     (* also disjointness of fpl and fpf *)
-    sound_state (Callstate vf args k bor_stk m)
-| sound_returnstate: forall sg fpf m k retty rfp v bor_stk VMP MP
+    sound_state (Callstate fun_id args inout_fpm sup k)
+| sound_returnstate: forall sg k retty rfp inout_fpm sup
     (* For now, all function must have return type *)
     (RETY: typeof_cont_call (rs_sig_res sg) k = retty)
-    (WTVAL: sem_wt_val ce rfp v VMP)
-    (CAST: val_casted v retty)
-    (WTFP: wt_footprint ce retty rfp)
-    (COHERENT: coherent_fpf ce fpf MP)
-    (MPRED: m |= VMP ** MP)    
-    (STK: sound_stacks k bor_stk fpf),
+    (* (WTFP: wt_footprint ce retty rfp) *)
+    (STK: sound_stacks k),
     (** TODO: borrow check invariant is missing at function return *)
     (* (ACC: rsw_acc w (rsw sg flat_fp m Hm)), *)
-    sound_state (Returnstate v k bor_stk m)
+    sound_state (Returnstate rfp inout_fpm sup k)
 .
+
+(** Misc for invalidate_conflict_ref and kill_paths. TODO: merge with
+the related lemmas in BorrowCheckInv.v *)
+
+Ltac destr_if_with_name H name :=
+  match type of H with
+  | ((if ?x then _ else _) = _) =>
+      destruct x eqn: name; try congruence
+  end.
+
+
+Lemma get_owner_footprint_map_after_invalidate_ref: forall (fpm: fp_map) ph1 ph2 ak am fp,
+    get_owner_footprint_map ph1 (invalidate_conflict_ref_fpm ph2 ak am fpm) = OK fp ->
+    exists fp', get_owner_footprint_map ph1 fpm = OK fp'
+           /\ invalidate_conflict_ref ph2 ak am fp' = fp.
+Admitted.
+
+Lemma get_owner_path_map_after_invalidate_ref: forall (fpm: fp_map) ph1 ph2 ph vs ak am,
+    get_owner_path_map ph1 (invalidate_conflict_ref_fpm ph2 ak am fpm) = OK (ph, vs) ->
+    get_owner_path_map ph1 fpm = OK (ph, vs).    
+Admitted.
+
+Ltac destr_fp_map_elt p :=
+  destruct p as ((((?b & ?ofs) & ?r) & ?ty) & ?fp).
+
+Lemma fpm_to_orgm_after_invalidate_ref: forall (fpm: fp_map) ph ak am,
+    fpm_to_orgm (invalidate_conflict_ref_fpm ph ak am fpm) = fpm_to_orgm fpm.
+Proof.
+  intros. unfold fpm_to_orgm, invalidate_conflict_ref_fpm. 
+  eapply PTree.extensionality.
+  intros. erewrite ! PTree.gmap1.
+  destruct (fpm ! i); try destr_fp_map_elt p; auto.
+Qed.
+
+Lemma fpm_to_tenv_after_invalidate_ref: forall (fpm: fp_map) ph ak am,
+    fpm_to_tenv (invalidate_conflict_ref_fpm ph ak am fpm) = fpm_to_tenv fpm.
+Proof.
+  intros. unfold fpm_to_tenv, invalidate_conflict_ref_fpm. 
+  eapply PTree.extensionality.
+  intros. erewrite ! PTree.gmap1.
+  destruct (fpm ! i); try destr_fp_map_elt p; auto.
+Qed.
+
+
+(** invalidation of fp_ref preserves sound approximation invariant *)
+
+Lemma illegal_access_false_implies: forall le p am ak r ls,
+    illegal_access le p am ak = false ->
+    LOrgEnv.get r le = Live ls ->
+    conflict p ls am ak = false.
+Proof.
+  intros until ls. intros ILL.
+  unfold illegal_access in ILL.
+  erewrite PTree_Properties.exists_false in ILL. 
+  unfold LOrgEnv.get.
+  destruct (LOrgEnv.m le) ! (UnionFindDelete.UFD.repr (LOrgEnv.uf le) r) eqn: A; auto.  
+  - intros. subst. 
+    eapply ILL in A. unfold illegal_access_in_origin_state in A. 
+    destruct conflict; try congruence.
+  - intros. inv H.
+Qed.
+
+(* p is the path we access and p1 is the path in views *)
+Lemma loan_approx_conflict_loan_false_implies: forall p p1 am ak ln orgm ref_mut,
+    conflict_access ak ref_mut = true ->
+    conflict_loan p am ak ln = false ->
+    loan_approx orgm ln ref_mut p1 ->
+    relevant_path p am p1 = false.
+Proof.
+  intros until ref_mut. intros A1 A2 SOUND.
+  red in SOUND. unfold conflict_loan in A2.
+  destruct ln.
+  - destruct (extern_loc_region orgm p1); try contradiction.
+    destr_path_of_place p0. destruct p1 as (id2 & pj2) eqn: P1.
+    destruct SOUND as (B1 & B2 & B3). subst.
+    assert (C: conflict_access ak mut = true).
+    { destruct ak; destruct ref_mut; simpl in A1; try congruence; destruct mut; simpl in B3; simpl; auto. }
+    rewrite C in A2. 
+    destruct (relevant_place p p0 am) eqn: C1; simpl in A2; try congruence.   
+    (* C1 implies: p0 -> p (p0 is prefix of p) or p ->(am) p0 is false;
+       B2 (the loans we analyze approximates the real view) implies: p0 -> (id2,phl) (p0 is prefix of (id2, phl), i.e., p1) *)
+    destruct (is_prefix_strict_path (id2, pj2) p) eqn: PREFIX.
+    (* we have p0 -> (id2, phl) -> p, which is contradict to [p0 -> p
+    is false] implies by C1 *)
+    + admit.
+    + unfold relevant_path, relevant_place in *. 
+      rewrite PREFIX.
+      destruct (match am with
+                | Ashallow => is_shallow_prefix_path p (id2, pj2)
+                | Adeep => is_prefix_path p (id2, pj2)
+                end) eqn: PRE_AM; auto.
+      (* Since we have [p ->(am) p0 = false] and [p0 -> (id2, phl)], we
+      have [p -> (am) (id2,phl) = false]. Prove by contradiction? If [p
+      -> (am) (id2,phl) = true] and [p0 -> (id2, phl)] then we have
+      either [p0 is prefix of p] or [p is support prefix of p0]. THe
+      former case is contradict with [PREFIX] and the latter case is
+      contradict with [p ->(am) p0 = false]. *)
+      assert (CONTR: match am with
+                     | Ashallow => is_shallow_prefix p p0
+                     | Adeep => is_support_prefix p p0
+                     end = true).
+      { admit. }
+      rewrite CONTR in C1. rewrite orb_true_r in C1. congruence.
+  - destruct (extern_loc_region orgm p1); try contradiction. subst.
+    (** TODO: p1 is an external access path, so p (which is a local
+    place) cannot be prefix or decendant of p1. But this lemma does
+    not give this premises. *)
+    admit.
+
+Admitted.
+
+Lemma loans_approx_views_not_conflict: forall vs p am ak ref_mut ls orgm
+  (SOUND: loans_approx_views orgm ls ref_mut vs)
+  (CONFLICT: conflict p ls am ak = false),
+    conflict_access ak ref_mut && conflict_view p am vs = false.
+Proof.
+  induction vs; intros.
+  - simpl. ring.
+  - unfold loans_approx_views, conflict, conflict_view in *. 
+    exploit IHvs. intros. eapply SOUND. right. auto.
+    eauto. intros A.
+    (* Proof idea: the target is to prove that [relevant_path p am a =
+    false]. We know for each loan in the loans set which approx
+    (a::vs), there is no conflict loan w.r.t. p under am and ak. But
+    [conflict_loan p am ak ln = false] may be derived from the fact
+    that [conflict_access ak (mut of the relevant_place in ln)] is
+    false (the opposite case is the normal case which may be proved by
+    loan_approx). But we need to prove that it is impossible. How?
+    First, we can only consider the case [conflict_access ak ref_mut =
+    true]. Then, since [loan_approx orgm ln ref_mut a], there exists a
+    relevant path in ln w.r.t. [p] must have matched mutability with
+    [ref_mut]. It further means that there exists a relevant place in
+    [ln] w.r.t. [p] must have matched mutability with [ref_mut], which
+    can further derive that [conflict_access ak (mut of this
+    relevant_place in ln)] is true. *)
+    (* We first say that [conflict_access ak ref_mut] is true *)
+    destruct (conflict_access ak ref_mut) eqn: C1; simpl in *; auto.
+    rewrite A. rewrite orb_false_r.
+    (* prove relevant_path p am a = false *)
+    eapply negb_false_iff in CONFLICT.
+    eapply LoanSet.for_all_2 in CONFLICT.
+    2: { red. unfold Proper. reflexivity. }
+    exploit (SOUND a). auto.
+    intros (ln & A1 & A2).
+    eapply CONFLICT in A1. eapply negb_true_iff in A1.
+    eapply loan_approx_conflict_loan_false_implies; eauto.
+Qed.      
+  
+
+
+Lemma invalidate_conflict_ref_fpm_preserves_borchk_approx: forall fpm p am ak le live
+    (SOUND: sound_loan_analysis ce live le fpm)
+    (ILL_ACCESS: illegal_access le p am ak = false),
+    sound_loan_analysis ce live le (invalidate_conflict_ref_fpm p ak am fpm).
+Proof.
+  intros. red. intros.
+  exploit get_owner_path_map_after_invalidate_ref; eauto. intros GET_PH1.
+  (** The most important property we need to prove is that opt_ph in
+  GET_FP may not be the same as the opt_ph in fpm because of the
+  invalidation, but we need to prove that they are the same using the
+  checking result of [illegal_access] *)  
+  exploit (@get_owner_footprint_map_after_invalidate_ref); eauto.
+  intros (fp1 & GET_FP1 & INVREF).
+  destruct fp1; inv INVREF.  
+  (* use sound approximation in fpm to prove that ph0 is not invalid *)
+  erewrite !fpm_to_orgm_after_invalidate_ref, !fpm_to_tenv_after_invalidate_ref in *.
+  exploit SOUND; eauto. 
+  intros (ls & A1 & (rph & A2) & A3). subst.
+  exists ls. split; eauto.
+  split; auto. 
+  exists rph.
+  exploit illegal_access_false_implies; eauto. intros CONFLICT_FALSE.
+  erewrite loans_approx_views_not_conflict; eauto.
+Qed.
+
+
+(** evaluation of expression preserves invariant *)
+
+
+Lemma eval_expr_preserves_borchk_approx: forall e fpm1 fpm2 live le vfp
+  (BORROW_APPROX: sound_loan_analysis ce live le fpm1)
+  (EVAL: eval_expr ce fpm1 e = OK (vfp, fpm2))
+  (* It ensures that we do not invalidate some reference (which is
+  live) incorrectly. *) 
+  (BORROW_CHECK: check_expr le e = OK tt)
+  (WT: wt_expr (fpm_to_env fpm1) ce e),
+    sound_loan_analysis ce live le fpm2
+    /\ sound_loan_analysis_footprint ce le fpm2 vfp (typeof e).
+Proof.
+  intros. destruct e.  
+  (* moveplace *)
+  - simpl in EVAL. monadInv EVAL.
+    destruct x.
+    simpl in BORROW_CHECK.
+    destr_if_with_name BORROW_CHECK ILL_ACCESS.
+    (** TODO: add premise about that p is a local place*)
+    eapply invalidate_conflict_ref_fpm_preserves_borchk_approx with (p:= p) (am:= Adeep) (ak:= AWrite) in BORROW_APPROX as BORROW_APPROX1; eauto.
+
+
+Ltac simpl_getIM IM :=
+  generalize IM as IM1; intros;
+  inversion IM1 as [? | ? | ? ? GETINIT GETUNINIT]; subst;
+  try rewrite <- GETINIT in *; try rewrite <- GETUNINIT in *.
+
+Lemma step_preservation: forall s1 t s2,
+    sound_state s1 ->
+    Step L s1 t s2 ->
+    sound_state s2.
+Proof.
+  intros s1 t s2 SOUND STEP. inv STEP.
+  (* Sassign *)
+  - inv SOUND. inv MCK_STMT. inv BORCK_STMT.
+    (* unfold move check and borrow check result. TODO: write ltac for these unfold code *)
+    simpl in TR. simpl_getIM IM.
+    destruct (move_check_expr ce mayinit mayuninit universe e) eqn: MOVE1; try congruence.
+    unfold move_check_expr in MOVE1.
+    destruct (move_check_expr' ce mayinit mayuninit universe e) eqn: MOVECKE; try congruence.
+    destruct p0 as (mayinit' & mayuninit').
+    destruct (move_check_assign mayinit' mayuninit' universe p) eqn: MOVE2; try congruence.
+    inv TR.
+    simpl in TR0. rewrite LOANS_ST in TR0. 
+    unfold BorrowCheckPolonius.borrow_check_stmt, borrow_check_stmt_aux, check_assignment in TR0.
+    monadInv TR0. monadInv EQ.
+    rename EQ0 into BORCK_EXPR. rename EQ1 into BORCKP.
+    (* end of unfold *)
+    set (live_st := (RegionLiveness.transfer f cfg (regset_fun f) pc live !! pc)) in *.
+    set (loans_env1 := (LOrgEnv.apply_liveness live_st loans_env)) in *.
+    assert (LIVE_EQ: live_st = reg_expr_live e (reg_assign_place p (live!!pc))).
+    { unfold live_st. unfold RegionLiveness.transfer. rewrite SEL.
+      rewrite STMT. reflexivity. }
+    (** how to show that the regions in [e] and [p] are live, so that
+    we can use the borrow check invariant *)
+    (* evaluate expr *)
+    exploit eval_expr_match. eauto. eapply MPRED. 
+    eapply BORCK_INV. all: eauto. admit.
+    intros (tv & tfp & fpm2 & mp1 & mp2 & TEVAL & FPMEQ & WTVAL & MEQ1 & COH1 & A1 & A2).
+    (* evaluate assignee place: before that, we need to prove moving a
+    place in the evaluation of expression preserve the borrow check
+    invariant for the sv_map and fp_map *)
+
+Admitted.
+
